code/nacl-box/Hacl.NaCl.Box.fst
@@ -1,0 +1,77 @@
+module Hacl.NaCl.Box
+
+module ST = FStar.HyperStack.ST
+open FStar.HyperStack.All
+open FStar.HyperStack
+open FStar.Mul
+
+open Lib.IntTypes
+open Lib.Buffer
+open Lib.ByteBuffer
+
+module Spec = Spec.Box
+module LibSeq = Lib.Sequence
+
+val crypto_box_detached: c:buffer uint8 -> tag:lbuffer uint8 16ul -> m:buffer uint8 ->
+			 mlen:size_t{length c = v mlen /\ length m = v mlen} ->
+			 n:lbuffer uint8 24ul -> pk:lbuffer uint8 32ul -> sk:lbuffer uint8 32ul ->
+   			 Stack size_t
+			 (requires (fun h -> live h c /\ live h m /\ live h sk /\ live h pk /\ live h n /\ live h tag /\
+					  disjoint tag c /\ eq_or_disjoint (m <: lbuffer uint8 mlen) (c <: lbuffer uint8 mlen)))
+			 (ensures (fun h0 _ h1 -> modifies (loc c |+| loc tag) h0 h1))
+			(*
+			/\
+			  (as_seq h1 tag,as_seq h1 c) ==
+			   Spec.box_detached (as_seq h0 sk) (as_seq h0 pk) (as_seq h0 n) (as_seq h0 m))) *)
+#set-options "--z3rlimit  300"
+let crypto_box_detached c tag m mlen n pk sk =
+  Hacl.Impl.Box.box_detached mlen c tag sk pk n m;
+  0ul
+
+
+
+val crypto_box_open_detached: m:buffer uint8 -> c:buffer uint8 -> tag:lbuffer uint8 16ul ->
+			 mlen:size_t{length c = v mlen /\ length m = v mlen} ->
+			 n:lbuffer uint8 24ul -> pk:lbuffer uint8 32ul -> sk:lbuffer uint8 32ul ->
+			Stack size_t
+			(requires (fun h -> live h c /\ live h m /\ live h pk /\ live h sk /\ live h n /\ live h tag /\
+				   disjoint tag c /\ eq_or_disjoint (m <: lbuffer uint8 mlen) (c <: lbuffer uint8 mlen)))
+			(ensures (fun h0 _ h1 -> modifies (loc m) h0 h1))
+			(*
+			/\
+			  (as_seq h1 tag,as_seq h1 m) ==
+			   Spec.box_open_detached (as_seq h0 pk) (as_seq h0 sk) (as_seq h0 n) (as_seq h0 tag) (as_seq h0 c))) *)
+let crypto_box_open_detached m c tag mlen n pk sk =
+    Hacl.Impl.Box.box_open_detached mlen m pk sk n c tag
+
+val crypto_box_easy: c:buffer uint8 -> m:buffer uint8 ->
+		     mlen:size_t{length c = v mlen + 16 /\ length m = v mlen} ->
+		     n:lbuffer uint8 24ul -> pk:lbuffer uint8 32ul -> sk:lbuffer uint8 32ul ->
+ 		     Stack size_t
+		     (requires (fun h -> live h c /\ live h m /\ live h sk /\ live h pk /\ live h n /\
+				      disjoint (m <: lbuffer uint8 mlen) (c <: lbuffer uint8 mlen)))
+		     (ensures (fun h0 _ h1 -> modifies (loc c) h0 h1))
+			(*
+			/\
+			  as_seq h1 c ==
+			   Spec.box_easy (as_seq h0 sk) (as_seq h0 pk) (as_seq h0 n) (as_seq h0 m))) *)
+let crypto_box_easy c m mlen n pk sk =
+  Hacl.Impl.Box.box_easy mlen c sk pk n m;
+  0ul
+
+
+val crypto_box_open_easy: m:buffer uint8 -> c:buffer uint8 ->
+			 mlen:size_t{length c = v mlen + 16 /\ length m = v mlen} ->
+			 n:lbuffer uint8 24ul -> pk:lbuffer uint8 32ul -> sk:lbuffer uint8 32ul ->
+			Stack size_t
+			(requires (fun h -> live h c /\ live h m /\ live h pk /\ live h sk /\ live h n /\
+				   disjoint (m <: lbuffer uint8 mlen) (c <: lbuffer uint8 mlen)))
+			(ensures (fun h0 _ h1 -> modifies (loc m) h0 h1))
+			(*
+			/\
+			   as_seq h1 m ==
+			   Spec.box_open_easy (as_seq h0 pk) (as_seq h0 sk) (as_seq h0 n) (as_seq h0 c))) *)
+let crypto_box_open_easy m c mlen n pk sk =
+    Hacl.Impl.Box.box_open_easy mlen m pk sk n c 
+
+
